 Solve the following system of linear equations.
 \begin{multicols}{2}
\begin{enumerate}[label=\thesubsection.\arabic*,ref=\thesubsection.\theenumi]
\item 
 \begin{align*}2x+5y&=1\\ 3x+2y&=7\end{align*}
\item \begin{align*}
	5x-4y+8&=0\\ 
      	7x+6y-9&=0
	\end{align*}
\item \begin{align*}
	9x+3y+12&=0\\
	18x+6y+24&=0
	\end{align*}
\item \begin{align*}
        6x-3y+10&=0\\
	2x-y+9&=0
	\end{align*}
	\item \begin{align*}
       		3x+2y&=5 \\
      		2x-3y&=7
    	       \end{align*} 
	\item \begin{align*}
		2x-3y&=8\\
		4x-6y&=9
		\end{align*}
	\item \begin{align*}
		\frac{3}{2}x+\frac{5}{3}y&=7\\
		9x-10y&=14
		\end{align*}
\item \begin{align*}
		5x-3y&=11\\
		-10x+6y&=-22
	\end{align*}
\item \begin{align*}
         \frac{4}{3}x+2y&=8\\
	  2x+3y&=12
	\end{align*}
\item \begin{align*}
	x+y&=5\\
	2x+y&=10
	\end{align*}
\item \begin{align*}
	x-y&=8\\
	3x-3y&=16
	\end{align*}
\item \begin{align*}
 	2x+y-6&=0\\
 	4x-2y+4&=0
	\end{align*}
\item \begin{align*}
	2x-2y-2&=0\\
	4x-4y-5&=0
	\end{align*}
	\item \begin{align*}
	x-3y-3&=0\\
	3x-9y-2&=0
        \end{align*}
       \item \begin{align*}
	2x+y&=5\\
	3x+2y&=8
	\end{align*}
	\item \begin{align*}
	3x-5y&=20\\
	6x-10y&=40
	\end{align*}
	\item \begin{align*}
	x-3y-7&=0\\
	3x-3y-15&=0
        \end{align*}
\item \begin{align*}
8x+5y&=9
\\ 3x+2y&=4
\end{align*}
	\item
	\begin{align*}
   	 x+y&=14 \\x-y&=4
	\end{align*}
	\item
	\begin{align*}
    	3x-y&=3\\ 9x-3y&=9
	\end{align*}
\item 	\begin{align*}   	
 	02x+03y&=13\\ 04x+05y&=23
	\end{align*}
	\item     
	\begin{align*}
	\sqrt{2x}+\sqrt{3y}&=0\\ \sqrt{3x}-\sqrt{8y}&=0
	\end{align*}
	\item
	\begin{align*}
    	\frac{3x}{2}-\frac{5y}{2}&=-2\\ \frac{x}{3}+\frac{y}{2}&=\frac{13}{6}
    	\end{align*}
\item
\begin{align*}
px+qy&=p-q\\ qx-py&=p+q
\end{align*}
\item
\begin{align*}                                                   
ax+by&=c\\ bx+ay&=1+c
\end{align*}
\item 
\begin{align*}
\frac {x}{a}-\frac{y}{b}&=0\\ ax+by&=a^2+b^2
\end{align*}
\item
\begin{align*}
(a-b)x+(a+b)y&=a^2-2ab-b^2\\ (a+b)(x+y)&=a^2+b^2
\end{align*}
\item
\begin{align*}
152x-378y&=-74\\ -378x+152y&=-604
\end{align*}
\item
	\begin{align*}
5x-8y+1 &= 0 \\ 3x-\frac{24}{5}y+\frac{3}{5} &= 0
\end{align*}
\item 
	\begin{align*}
x+3y &= 6 \\  2x-3y &= 12
\end{align*}
\item 
	\begin{align*}
7x-15y &= 2 \\  x+2y &= 3
\end{align*}
\item 
\begin{align*}
2x+3y &= 8 \\ 4x+6y &= 7
\end{align*}
\item \begin{align*}x+2y-4&=0\\2x+4y-12&=0\end{align*}
\item \begin{align*}x+2y-4&=0\\2x+4y-12&=0\end{align*}
\item \begin{align*}x+y&=5\\2x-3y&=4\end{align*}
\item \begin{align*}3x+4y&=10\\ 2x-2y&=2\end{align*}
\item \begin{align*}3x-5y-4&=0\\9x&=2y+7\end{align*}
\item \begin{align*}\frac{x}{2}+\frac{2y}{3}&=-1\\x-\frac{y}{3}&=0\end{align*}
\item
\begin{align*}
\frac{1}{2x}+\frac{1}{3y}&=2 \\ \frac{1}{3x}+\frac{1}{2y}&=\frac{13}{6}
\end{align*}
\item
\begin{align*}
\frac{2}{\sqrt{x}}+\frac{3}{\sqrt{y}}&=2\\
\frac{4}{\sqrt{x}}-\frac{9}{\sqrt{y}}&=-1
\end{align*}
\item
\begin{align*}
\frac{4}{x}+3y&=14\\ \frac{3}{x}-4y&=23
\end{align*}
\item
\begin{align*}
\frac{5}{x-1}+\frac{1}{y-2}&=2\\ \frac{6}{x-1}-\frac{3}{y-2}&=1
\end{align*}
\item
\begin{align*}
\frac{7x-2y}{xy}&=5\\ \frac{8x+7y}{xy}&=15
\end{align*}
\item
\begin{align*}
6x+3y&=6xy\\ 2x+4y&=5xy
\end{align*}
\item
\begin{align*}
\frac{10}{x+y}+\frac{2}{x-y}&=4\\ \frac{15}{x+y}-\frac{5}{x-y}&=-2
\end{align*}
\item
\begin{align*}
\frac{1}{3x+y}+\frac{1}{3x-y}&=\frac{3}{4}\\ \frac{1}{2(3x+y)}-\frac{1}{2(3x-y)}&=\frac{-1}{8}
\end{align*}
\item  
\begin{align*}
 x+2y &= 2\\
2x+3y &= 3
\end{align*}
\item
\begin{align*}
 2x-y &= 5\\
 x+y &= 4
\end{align*}
\item
\begin{align*}
 x+3y &= 5\\
 2x+6y&= 8
\end{align*}
\item
\begin{align*}
 x+y+z &= 1\\
 2x+3y+2z &= 2\\
 ax+ay+2az &= 4
\end{align*}
\item
\begin{align*}
 3x-y-2z &= 2\\
 2y-z &= -1\\
 3x-5y &= 3
\end{align*}
\item 
\begin{align*}
 5x-y+4z &= 5\\
 2x+3y+5z &= 2\\
 5x-2y+6z &= -1
\end{align*}
\item   
\begin{align*}
5x+2y &= 4\\
7x+3y &= 5
\end{align*}
\item 
\begin{align*}
 2x-y &= -2\\
 3x+4y &= 3
\end{align*}
\item
\begin{align*}
 4x-3y &= 3\\
 3x-5y &= 7
\end{align*}
\item
\begin{align*} 
 5x+2y &= 3\\
 3x+2y &= 5
\end{align*}
\item 
\begin{align*}
\frac{2}{x}+\frac{3}{y}&= 13 \\ \frac{5}{x}+\frac{4}{y} &= -2
\end{align*}
\item 
\begin{align*}
\frac{5}{x-1}+\frac{1}{y-2}&= 2 \\ \frac{6}{x-1}-\frac{3}{y-2}&= 1
\end{align*}
\item
\begin{align*}
 2x+y+z &= 1\\
 x-2y-z &= \frac{3}{2} \\
 3y-5z &= 9
\end{align*}
\item
\begin{align*}
 x-y+z &= 4\\
 2x+y-3z &= 0\\
 x+y+z &= 2
\end{align*}
\item
\begin{align*}
 2x+3y+3z &= 5\\
 x-2y+z &= -4\\
 3x-y-2z &= 3
\end{align*}
\item   \label{prob:14}
\begin{align*}
 x-y+2z &= 7\\
 3x+4y-5z &= -5\\
 2x-y+3z &= 12
\end{align*}
\item  
\begin{align*}
x-y+2z&=1\\ 2z-3z&=1\\ 3x-2y+4z&=2
\end{align*}
\item 
\begin{align*}
3x-2y+3z&=8\\ 2x+y-z&=1\\ 4x-3y+2z&=4
\end{align*}
\item Solve
\begin{align*}
\myvec
{x+y+z \\ x+z \\ y+z }=
\myvec{9 \\ 5 \\  7}
\end{align*}
\item 
\begin{align*}
	\vec{X}+\vec{Y}&= \myvec
{7 & 0 \\ 2 & 5} 
\\
		\vec{X}-\vec{Y}&=\myvec
{3 & 0 \\ 0 & 4}.
\end{align*}
\item  
\begin{align*}
\vec{X}+\vec{Y}=\myvec{5&2\\0&9}
	\\
\vec{X}-\vec{Y}=\myvec{3&6\\0&-1}
\end{align*}
\item 
\begin{align*}
	2\vec{X}+3\vec{Y}&=\myvec
{2 & 3 \\ 4 & 0}  
	\\
	3\vec{X}+2\vec{Y}&=\myvec
{2 & -2 \\ -1 & 5}
\end{align*}
\end{enumerate}
\end{multicols}
\begin{enumerate}[label=\thesubsection.\arabic*,ref=\thesubsection.\theenumi,resume*]
%\item Find $\vec{X}$ and $\vec{Y}$, if
\item If 
\begin{align}
	x \myvec
{2 \\ 3} + y \myvec
{-1 \\ 1}= \myvec
{10 \\ 5}
\end{align}
find the values of $x$ and $y$.
\item Solve $2x+3y=11$ and $2x+4y=-24$ and hence find the value of $m$ for which $y=mx+3$.
\item For which values of $p$ does the pair of equations given below have a unique solution.
\begin{align}
4x+py+8 = 0 \\ 2x+2y+2 = 0
\end{align}
\item For what values of $k$ will the following pair of linear equations have infinitely many solutions.
\begin{align}
kx+3y-(k-3) = 0 \\ 12x+ky-k = 0
\end{align}
\item Find the values of $a, b, c$ and $d$ from the following equation 
\begin{align} 
\myvec{2a+b&a-2b\\5c-d&4c+d} = \myvec{4&-3\\11&24} 
\end{align}
\end{enumerate}
